Make [GPointers] based off of [GPointersViaRefs]

Gpointers.fst
@@ -51,8 +51,8 @@ assume val ptr_eq:
 
 let disjoint (#t:Type) (a b: gpointer t) = B.disjoint a b
 
-unfold let is_null (p:gpointer_or_null 't) = CN.is_null p
-unfold let is_not_null (p:gpointer_or_null 't) = not (CN.is_null p)
+unfold let is_null (p:gpointer_or_null 't) = B.length p = 0
+unfold let is_not_null (p:gpointer_or_null 't) = B.length p <> 0
 
 assume val null : #t:Type -> gnull t
 
@@ -60,10 +60,60 @@ let test_null #t =
   let p : gpointer_or_null t = null in
   assert (is_null p)
 
-open C.Nullity
-open FStar.Buffer
+unfold let ( := ) (a:gpointer 't) (b:'t) = B.(a.(0ul) <- b)
+unfold let ( ! ) (a:gpointer 't) = B.index a 0ul
 
-unfold let ( := ) (a:gpointer 't) (b:'t) = a.(0ul) <- b
-unfold let ( ! ) (a:gpointer 't) = !* a
+unfold let recall (#t:Type) (p: gpointer_or_null t) = B.recall p
 
-unfold let recall (#t:Type) (p: gpointer_or_null t) = recall p
+val non_null:
+  #t:Type ->
+  a:gpointer_or_null t{is_not_null a} ->
+  b:gpointer t
+let non_null #t a = a
+
+val lemma_non_null :
+  #t:Type ->
+  a:gpointer_or_null t{is_not_null a} ->
+  Lemma (ensures (a == non_null a))
+    [SMTPat (non_null a)]
+let lemma_non_null #t a = ()
+
+val of_non_null:
+  #t:Type ->
+  a:gpointer t ->
+  b:gpointer_or_null t
+let of_non_null #t a = a
+
+val lemma_of_non_null:
+  #t:Type ->
+  a:gpointer t ->
+  Lemma (ensures (is_not_null (of_non_null a)) /\ (of_non_null a == a))
+let lemma_of_non_null #t a = ()
+
+let heap = HS.mem
+let contains = B.live
+
+unfold let (@) (a:gpointer 't) (h0:heap{h0 `contains` a}) = B.get h0 a 0
+unfold let (^@) (a:gpointer_or_null 't{is_not_null a}) (h0:heap{h0 `contains` (non_null a)}) = (non_null a) @ h0
+
+let (==$) (#t:Type) (a:gpointer_or_null t) (b:gpointer t) =
+  is_not_null a /\
+  (let (a:_{is_not_null a}) = a in // workaround for not using two phase type checker
+   g_ptr_eq (non_null a) b)
+
+// logic : Cannot use due to https://github.com/FStarLang/FStar/issues/638
+let not_aliased (#t:Type) (a:gpointer_or_null t) (b:gpointer_or_null t) : GTot Type0 =
+  is_null a \/ is_null b \/
+  (let (a:_{is_not_null a}) = a in // workaround for not using two phase type checker
+   let (b:_{is_not_null b}) = b in
+   disjoint (non_null a) (non_null b))
+
+// logic : Cannot use due to https://github.com/FStarLang/FStar/issues/638
+let not_aliased0 (#t:Type) (a:gpointer t) (b:gpointer_or_null t) : GTot Type0 =
+  is_null b \/
+  (let (b:_{is_not_null b}) = b in // workaround for not using two phase type checker
+   disjoint a (non_null b))
+
+logic
+let not_aliased00 (#t:Type) (a:gpointer t) (b:gpointer t) : GTot Type0 =
+  disjoint a b
